IMP--_To_SAS+/Domains.thy
@@ -1,0 +1,97 @@
+\<^marker>\<open>creator Florian Keßler\<close>
+
+section "Domains"
+
+theory Domains imports "../IMP--/Small_StepT" 
+begin
+
+fun max_constant :: "com \<Rightarrow> nat" where
+"max_constant SKIP = 0" |
+"max_constant (Assign vname aexp) = (case aexp of
+  (A a) \<Rightarrow> (case a of (V var) \<Rightarrow> 0 | (N val) \<Rightarrow> val) |
+  (Plus a b) \<Rightarrow> b |
+  (Sub a b) \<Rightarrow> b)" |
+"max_constant (Seq c1  c2) = max (max_constant c1) (max_constant c2)" |         
+"max_constant (If _ c1 c2) = max (max_constant c1) (max_constant c2)"  |   
+"max_constant (While _ c) = max_constant c"
+
+lemma step_cant_increase_max_constant: "(c1, s1) \<rightarrow> (c2, s2) \<Longrightarrow> max_constant c1 \<ge> max_constant c2"
+proof (induction c1 arbitrary: s1 c2 s2)
+  case (Seq c11 c12)
+  then show ?case by force
+qed auto
+
+lemma execution_cant_increase_max_constant: "(c1, s1) \<rightarrow>\<^bsup> t \<^esup> (c2, s2)
+   \<Longrightarrow> max_constant c1 \<ge> max_constant c2"
+proof (induction t c1 s1 c2 s2 rule: rel_pow_induct)
+next
+  case (step a b a b n a b)
+  then show ?case using step_cant_increase_max_constant by fastforce
+qed auto
+
+lemma [simp]: "\<exists>y. nat \<bar>int (s x) - int (s y)\<bar> \<le> z"
+proof
+  show "nat \<bar>int (s x) - int (s x)\<bar> \<le> z" by auto
+qed
+
+lemma [simp]: "\<exists>y. nat \<bar>int (s x) + int z - int (s y)\<bar> \<le> z"
+proof
+  show "nat \<bar>int (s x) + int z - int (s x)\<bar> \<le> z" by auto
+qed
+
+lemma [simp]: "\<exists>y. nat \<bar>int (s x - z) - int (s y)\<bar> \<le> z" 
+proof
+  show "nat \<bar>int (s x - z) - int (s x)\<bar> \<le> z" by auto
+qed
+
+lemma exists_bigger_helper: "a \<le> b \<Longrightarrow> (\<exists>v2. nat \<bar>int (s' v1) - int (s v2)\<bar> \<le> a)
+   \<Longrightarrow>  (\<exists>v2. nat \<bar>int (s' v1) - int (s v2)\<bar> \<le> b)"
+  using le_trans by blast
+
+lemma register_change_single_step_bound: "(c1, s1) \<rightarrow> (c2, s2) 
+  \<Longrightarrow> (s2 v1 \<le> max_constant c1) \<or> (\<exists>v2. nat \<bar>(int (s2 v1)) - (int (s1 v2))\<bar> \<le> max_constant c1)"
+proof (induction c1 s1 c2 s2 rule: small_step.induct[split_format(complete)])
+next
+  case (Seq2 c\<^sub>1 s c\<^sub>1' s' c\<^sub>2)
+  have "s' v1 \<le> max_constant (c\<^sub>1 ;; c\<^sub>2) \<or> (\<exists>v2. nat \<bar>int (s' v1) - int (s v2)\<bar> \<le> max_constant c\<^sub>1)" 
+    using Seq2 by auto
+  then show ?case
+  proof (elim disjE)
+    assume "(\<exists>v2. nat \<bar>int (s' v1) - int (s v2)\<bar> \<le> max_constant c\<^sub>1)"
+    moreover have *: "max_constant c\<^sub>1 \<le> max_constant (c\<^sub>1 ;; c\<^sub>2)" by auto
+    ultimately show ?thesis using Seq2 exists_bigger_helper[OF *] by metis
+  qed auto
+qed (auto split: aexp.splits atomExp.splits) 
+
+lemma register_change_bounded:
+   "(c1, s1) \<rightarrow>\<^bsup>t\<^esup> (c2, s2) \<Longrightarrow> (s2 v1 \<le>  t * (max_constant c1)) \<or> 
+             (\<exists>v2. nat \<bar>(int (s2 v1)) - (int (s1 v2))\<bar> \<le> t * (max_constant c1))"
+proof (induction t arbitrary: c2 s2 v1)
+  case (Suc t)
+  then obtain c1' s1' where *: "((c1, s1) \<rightarrow>\<^bsup> t \<^esup> (c1', s1')) \<and> ((c1', s1') \<rightarrow> (c2, s2))"
+    using rel_pow_Suc_E by (metis old.prod.exhaust)
+  then have "(s2 v1 \<le>  max_constant c1') \<or> (\<exists>v2. nat \<bar>(int (s2 v1)) - (int (s1' v2))\<bar> \<le> max_constant c1')"
+    using register_change_single_step_bound by blast
+  then show ?case
+  proof (elim disjE)
+    assume "s2 v1 \<le> max_constant c1'"
+    then show ?thesis using * execution_cant_increase_max_constant by fastforce
+  next
+    assume "\<exists>v2. nat \<bar>(int (s2 v1)) - (int (s1' v2))\<bar> \<le> max_constant c1'"
+    then obtain v2 where v2_def: "nat \<bar>(int (s2 v1)) - (int (s1' v2))\<bar> \<le> max_constant c1'" by blast
+    then have "s1' v2 \<le> t * max_constant c1 \<or>
+      (\<exists>v3. nat \<bar>int (s1' v2) - int (s1 v3)\<bar> \<le> t * max_constant c1)" using Suc * by blast
+    then show ?thesis
+    proof (elim disjE)
+      assume "s1' v2 \<le> t * max_constant c1"
+      then show ?thesis using execution_cant_increase_max_constant * v2_def by fastforce
+    next
+      assume "\<exists>v3. nat \<bar>int (s1' v2) - int (s1 v3)\<bar> \<le> t * max_constant c1"
+      moreover then obtain v3 where "nat \<bar>int (s1' v2) - int (s1 v3)\<bar> \<le> t * max_constant c1" by blast
+      ultimately have "nat \<bar>int (s2 v1) - int (s1 v3)\<bar> \<le> (t + 1) * max_constant c1"  
+        using execution_cant_increase_max_constant * v2_def by fastforce
+      then show ?thesis by auto
+    qed
+  qed
+qed auto
+end
